lib/concurrency: improve style
Signed-off-by: Corey Lewis <corey.lewis@proofcraft.systems>

lib/concurrency/Triv_Refinement.thy
@@ -4,23 +4,20 @@
  * SPDX-License-Identifier: BSD-2-Clause
  *)
 theory Triv_Refinement
-
-imports
-  "Monads.Trace_More_RG"
-  "Monads.Trace_Strengthen_Setup"
-
+  imports
+    "Monads.Trace_More_RG"
+    "Monads.Trace_Strengthen_Setup"
 begin
 
-text \<open>This is a simple (almost trivial) definition of refinement,
-which simply resolves nondeterminism to a smaller set of options.\<close>
-definition
-  triv_refinement :: "('s,'a) tmonad \<Rightarrow> ('s,'a) tmonad \<Rightarrow> bool"
-where
+text \<open>
+  This is a simple (almost trivial) definition of refinement, which simply resolves nondeterminism
+  to a smaller set of options.\<close>
+definition triv_refinement :: "('s,'a) tmonad \<Rightarrow> ('s,'a) tmonad \<Rightarrow> bool" where
   "triv_refinement aprog cprog = (\<forall>s. cprog s \<subseteq> aprog s)"
 
 lemma triv_refinement_mono_bind:
   "triv_refinement a c \<Longrightarrow> triv_refinement (a >>= b) (c >>= b)"
-  "(\<forall>x. triv_refinement (b x) (d x)) \<Longrightarrow> triv_refinement (a >>= b) (a >>= d)"
+  "\<lbrakk>\<forall>x. triv_refinement (b x) (d x)\<rbrakk> \<Longrightarrow> triv_refinement (a >>= b) (a >>= d)"
    apply (simp add: triv_refinement_def bind_def)
    apply (intro allI UN_mono; simp)
   apply (simp only: triv_refinement_def bind_def' split_def)
@@ -29,14 +26,12 @@ lemma triv_refinement_mono_bind:
   done
 
 lemma triv_refinement_trans:
-  "triv_refinement f g \<Longrightarrow> triv_refinement g h
-    \<Longrightarrow> triv_refinement f h"
+  "\<lbrakk>triv_refinement f g; triv_refinement g h\<rbrakk> \<Longrightarrow> triv_refinement f h"
   by (auto simp add: triv_refinement_def)
 
 lemma triv_refinement_bind:
-  "triv_refinement a c
-    \<Longrightarrow> (\<forall>x. triv_refinement (b x) (d x))
-    \<Longrightarrow> triv_refinement (bind a b) (bind c d)"
+  "\<lbrakk>triv_refinement a c; \<forall>x. triv_refinement (b x) (d x)\<rbrakk>
+   \<Longrightarrow> triv_refinement (bind a b) (bind c d)"
   by (metis triv_refinement_mono_bind triv_refinement_trans)
 
 lemma triv_refinement_mono_parallel:
@@ -52,11 +47,10 @@ lemma triv_refinement_mono_parallel':
   done
 
 lemma triv_refinement_parallel:
-  "triv_refinement a b
-    \<Longrightarrow> triv_refinement c d
-    \<Longrightarrow> triv_refinement (parallel a c) (parallel b d)"
+  "\<lbrakk>triv_refinement a b; triv_refinement c d\<rbrakk>
+   \<Longrightarrow> triv_refinement (parallel a c) (parallel b d)"
   by (metis triv_refinement_mono_parallel triv_refinement_mono_parallel'
-    triv_refinement_trans)
+            triv_refinement_trans)
 
 lemma select_subset:
   "(select S s \<subseteq> select S' s') = (S \<subseteq> S' \<and> (S \<noteq> {} \<longrightarrow> s = s'))"
@@ -71,34 +65,27 @@ lemma triv_refinement_select_eq:
   by (simp add: triv_refinement_def select_subset)
 
 lemma triv_refinement_rely:
-  "(\<And>s0 s. R' s0 s \<Longrightarrow> R s0 s) \<Longrightarrow>
-   triv_refinement (rely f R s0) (rely f R' s0)"
+  "\<lbrakk>\<And>s0 s. R' s0 s \<Longrightarrow> R s0 s\<rbrakk>
+   \<Longrightarrow> triv_refinement (rely f R s0) (rely f R' s0)"
   unfolding rely_def triv_refinement_def rely_cond_def
   by auto
 
 lemma triv_refinement_rely2:
-  "triv_refinement f g \<Longrightarrow>
-   triv_refinement (rely f R s0) (rely g R s0)"
+  "triv_refinement f g \<Longrightarrow> triv_refinement (rely f R s0) (rely g R s0)"
   unfolding rely_def triv_refinement_def rely_cond_def
   by auto
 
 lemma rely_rely_triv_refinement:
- "(\<And>s0 s. R s0 s \<Longrightarrow> R' s0 s) \<Longrightarrow>
- triv_refinement (rely f R' s0) (rely (rely f R s0) R' s0)"
+  "\<lbrakk>\<And>s0 s. R s0 s \<Longrightarrow> R' s0 s\<rbrakk> \<Longrightarrow> triv_refinement (rely f R' s0) (rely (rely f R s0) R' s0)"
   by (clarsimp simp: triv_refinement_def rely_def parallel_def)
 
 lemma validI_triv_refinement:
-  "triv_refinement f g
-    \<Longrightarrow> \<lbrace>P\<rbrace>,\<lbrace>R\<rbrace> f \<lbrace>G\<rbrace>,\<lbrace>Q\<rbrace>
-    \<Longrightarrow> prefix_closed g
-    \<Longrightarrow> \<lbrace>P\<rbrace>,\<lbrace>R\<rbrace> g \<lbrace>G\<rbrace>,\<lbrace>Q\<rbrace>"
+  "\<lbrakk>triv_refinement f g; \<lbrace>P\<rbrace>,\<lbrace>R\<rbrace> f \<lbrace>G\<rbrace>,\<lbrace>Q\<rbrace>; prefix_closed g\<rbrakk> \<Longrightarrow> \<lbrace>P\<rbrace>,\<lbrace>R\<rbrace> g \<lbrace>G\<rbrace>,\<lbrace>Q\<rbrace>"
   unfolding rely_def triv_refinement_def validI_def
   by fastforce
 
 lemma valid_triv_refinement:
-  "triv_refinement f g
-    \<Longrightarrow> \<lbrace>P\<rbrace> f \<lbrace>Q\<rbrace>
-    \<Longrightarrow> \<lbrace>P\<rbrace> g \<lbrace>Q\<rbrace>"
+  "\<lbrakk>triv_refinement f g; \<lbrace>P\<rbrace> f \<lbrace>Q\<rbrace>\<rbrakk> \<Longrightarrow> \<lbrace>P\<rbrace> g \<lbrace>Q\<rbrace>"
   unfolding rely_def triv_refinement_def valid_def mres_def
   by (fastforce elim: image_eqI[rotated])
 
@@ -107,16 +94,13 @@ lemma triv_refinement_refl:
   by (simp add: triv_refinement_def)
 
 lemma triv_refinement_select_concrete_All:
-  "\<forall>x \<in> S. triv_refinement aprog (cprog x)
-    \<Longrightarrow> triv_refinement aprog (select S >>= cprog)"
-  by (auto simp add: triv_refinement_def bind_def select_def)
+  "\<forall>x \<in> S. triv_refinement aprog (cprog x) \<Longrightarrow> triv_refinement aprog (select S >>= cprog)"
+  by (auto simp: triv_refinement_def bind_def select_def)
 
 lemma triv_refinement_select_abstract_x:
-  "x \<in> S \<Longrightarrow> triv_refinement (aprog x) cprog
-    \<Longrightarrow> triv_refinement (select S >>= aprog) cprog"
-  by (auto simp add: triv_refinement_def bind_def select_def)
+  "\<lbrakk>x \<in> S; triv_refinement (aprog x) cprog\<rbrakk> \<Longrightarrow> triv_refinement (select S >>= aprog) cprog"
+  by (auto simp: triv_refinement_def bind_def select_def)
 
-lemmas triv_refinement_elemD
-    = triv_refinement_def[THEN iffD1, rule_format, THEN subsetD]
+lemmas triv_refinement_elemD = triv_refinement_def[THEN iffD1, rule_format, THEN subsetD]
 
 end
